on utilise romega (gain de temps enORme). changement sur i2z
git-svn-id: svn://scm.gforge.inria.fr/svnroot/coq-contribs/trunk@360 0cf17b13-060f-0410-b1b1-c666bec9822a

Int.v
@@ -23,6 +23,7 @@
 *)
 
 Require Import ZArith. 
+Require Import ROmega. 
 
 Module Type Int.
 
@@ -138,15 +139,268 @@ Module Type Int.
   | H : _ |- _ => progress autorewrite with i2z in H; i2z
   | _ => try autorewrite with i2z
  end.
-
+(*
  Ltac iauto := i2z; auto with zarith.
  Ltac iomega := i2z; omega.
-
+*)
 End Int. 
 
 Module MoreInt (I:Int).
  Import I.
- Open Scope Z_scope.
+  
+  (* a reflexive version of the [i2z] tactic *)
+
+  Ltac i2z_gen := match goal with 
+    | |- (eq (A:=int) ?a ?b) => apply (i2z_eq a b); i2z_gen
+    | H : (eq (A:=int) ?a ?b) |- _ => 
+       generalize (f_equal i2z H); clear H; i2z_gen
+    | H : (eq (A:=Z) ?a ?b) |- _ => generalize H; clear H; i2z_gen
+    | H : (Zlt ?a ?b) |- _ => generalize H; clear H; i2z_gen
+    | H : (Zle ?a ?b) |- _ => generalize H; clear H; i2z_gen
+    | H : (Zgt ?a ?b) |- _ => generalize H; clear H; i2z_gen
+    | H : (Zge ?a ?b) |- _ => generalize H; clear H; i2z_gen
+    | H : _ -> ?X |- _ => match type of X with 
+       | Type => clear H; i2z_gen
+       | Prop => generalize H; clear H; i2z_gen
+      end
+    | H : _ <-> _ |- _ => generalize H; clear H; i2z_gen
+    | H : _ /\ _ |- _ => generalize H; clear H; i2z_gen
+    | H : _ \/ _ |- _ => generalize H; clear H; i2z_gen
+    | H : ~ _ |- _ => generalize H; clear H; i2z_gen
+    | _ => idtac
+   end.
+
+  Inductive ExprI : Set := 
+   | EI0 : ExprI
+   | EI1 : ExprI
+   | EI2 : ExprI 
+   | EI3 : ExprI
+   | EIplus : ExprI -> ExprI -> ExprI
+   | EIopp : ExprI -> ExprI
+   | EIminus : ExprI -> ExprI -> ExprI
+   | EImult : ExprI -> ExprI -> ExprI
+   | EImax : ExprI -> ExprI -> ExprI
+   | EIofZ : ExprZ -> ExprI
+   | EIraw : int -> ExprI
+  with 
+  ExprZ : Set := 
+   | EZplus : ExprZ -> ExprZ -> ExprZ
+   | EZopp : ExprZ -> ExprZ
+   | EZminus : ExprZ -> ExprZ -> ExprZ
+   | EZmult : ExprZ -> ExprZ -> ExprZ
+   | EZmax : ExprZ -> ExprZ -> ExprZ
+   | EZofI : ExprI -> ExprZ
+   | EZraw : Z -> ExprZ.
+
+  Inductive ExprP : Type := 
+   | EPeq : ExprZ -> ExprZ -> ExprP 
+   | EPlt : ExprZ -> ExprZ -> ExprP 
+   | EPle : ExprZ -> ExprZ -> ExprP 
+   | EPgt : ExprZ -> ExprZ -> ExprP 
+   | EPge : ExprZ -> ExprZ -> ExprP 
+   | EPimpl : ExprP -> ExprP -> ExprP
+   | EPequiv : ExprP -> ExprP -> ExprP
+   | EPand : ExprP -> ExprP -> ExprP
+   | EPor : ExprP -> ExprP -> ExprP
+   | EPneg : ExprP -> ExprP
+   | EPraw : Prop -> ExprP.
+
+Ltac interp_int trm := 
+ match constr:trm with 
+    | (plus ?X1 ?X2) => 
+        let e1 := interp_int X1 with e2 := interp_int X2 
+        in constr:(EIplus e1 e2)
+    | (minus ?X1 ?X2) => 
+       let e1 := interp_int X1 with e2 := interp_int X2 
+        in constr:(EIminus e1 e2)
+    | (mult ?X1 ?X2) => 
+       let e1 := interp_int X1 with e2 := interp_int X2 
+        in constr:(EImult e1 e2)
+    | (max ?X1 ?X2) => 
+       let e1 := interp_int X1 with e2 := interp_int X2 
+        in constr:(EImax e1 e2)
+    | (opp ?X1) => 
+        let e1 := interp_int X1 in constr:(EIopp e1)
+    | (_0) => constr:EI0
+    | (_1) => constr:EI1
+    | (_2) => constr:EI2
+    | (_3) => constr:EI3
+    | (z2i ?X1) => 
+        let e1 := interp_z X1 in constr:(EIofZ e1)
+    | ?X1 => constr:(EIraw X1)
+   end
+with interp_z trm := 
+   match constr:trm with 
+    | (Zplus ?X1 ?X2) => 
+        let e1 := interp_z X1 with e2 := interp_z X2 
+        in constr:(EZplus e1 e2)
+    | (Zminus ?X1 ?X2) => 
+        let e1 := interp_z X1 with e2 := interp_z X2 
+        in constr:(EZminus e1 e2)
+    | (Zmult ?X1 ?X2) => 
+        let e1 := interp_z X1 with e2 := interp_z X2 
+        in constr:(EZmult e1 e2)
+    | (Zmax ?X1 ?X2) => 
+        let e1 := interp_z X1 with e2 := interp_z X2 
+        in constr:(EZmax e1 e2)
+    | (Zopp ?X1) => 
+        let e1 := interp_z X1 in constr:(EZopp e1)
+    | (i2z ?X1) => 
+        let e1 := interp_int X1 in constr:(EZofI e1)
+    | ?X1 => constr:(EZraw X1)
+   end.
+
+Ltac interp_prop trm :=
+  match constr:trm with
+    | (?X1 <-> ?X2) => 
+        let e1 := interp_prop X1 with e2 := interp_prop X2 
+        in constr:(EPequiv e1 e2)
+    | (?X1 -> ?X2) => 
+        let e1 := interp_prop X1 with e2 := interp_prop X2 
+        in constr:(EPimpl e1 e2)
+    | (?X1 /\ ?X2) => 
+        let e1 := interp_prop X1 with e2 := interp_prop X2 
+        in constr:(EPand e1 e2)
+    | (?X1 \/ ?X2) => 
+        let e1 := interp_prop X1 with e2 := interp_prop X2 
+        in constr:(EPor e1 e2)
+    | (~ ?X1) =>
+        let e1 := interp_prop X1 in constr:(EPneg e1)
+    | (eq (A:=Z) ?X1 ?X2) => 
+        let e1 := interp_z X1 with e2 := interp_z X2 
+        in constr:(EPeq e1 e2)
+    | (Zlt ?X1 ?X2) =>
+        let e1 := interp_z X1 with e2 := interp_z X2 
+        in constr:(EPlt e1 e2)
+    | (Zle ?X1 ?X2) =>
+        let e1 := interp_z X1 with e2 := interp_z X2 
+        in constr:(EPle e1 e2)   
+    | (Zgt ?X1 ?X2) =>
+        let e1 := interp_z X1 with e2 := interp_z X2 
+        in constr:(EPgt e1 e2)   
+    | (Zge ?X1 ?X2) =>
+        let e1 := interp_z X1 with e2 := interp_z X2 
+        in constr:(EPge e1 e2)
+    | ?X1 =>  constr:(EPraw X1)
+   end.   
+
+Fixpoint interp_ExprI (e:ExprI) : int :=
+  match e with
+  | EI0 => _0
+  | EI1 => _1
+  | EI2 => _2
+  | EI3 => _3 
+  | EIplus e1 e2 => plus (interp_ExprI e1) (interp_ExprI e2)
+  | EIminus e1 e2 => minus (interp_ExprI e1) (interp_ExprI e2)
+  | EImult e1 e2 => mult (interp_ExprI e1) (interp_ExprI e2)
+  | EImax e1 e2 => max (interp_ExprI e1) (interp_ExprI e2)
+  | EIopp e1 => opp (interp_ExprI e1)
+  | EIofZ e1 => z2i (interp_ExprZ e1)
+  | EIraw i => i 
+  end 
+with interp_ExprZ (e:ExprZ) : Z := 
+ match e with 
+  | EZraw z => z
+  | EZplus e1 e2 => Zplus (interp_ExprZ e1) (interp_ExprZ e2)
+  | EZminus e1 e2 => Zminus (interp_ExprZ e1) (interp_ExprZ e2)
+  | EZmult e1 e2 => Zmult (interp_ExprZ e1) (interp_ExprZ e2)
+  | EZmax e1 e2 => Zmax (interp_ExprZ e1) (interp_ExprZ e2)
+  | EZopp e1 => Zopp (interp_ExprZ e1)
+  | EZofI e1 => i2z (interp_ExprI e1)
+  end.
+
+Fixpoint interp_ExprP (e:ExprP) : Prop := 
+ match e with 
+   | EPeq e1 e2 => (interp_ExprZ e1) = (interp_ExprZ e2)
+   | EPlt e1 e2 => Zlt (interp_ExprZ e1) (interp_ExprZ e2)
+   | EPle e1 e2 => Zle (interp_ExprZ e1) (interp_ExprZ e2)
+   | EPgt e1 e2 => Zgt (interp_ExprZ e1) (interp_ExprZ e2)
+   | EPge e1 e2 => Zge (interp_ExprZ e1) (interp_ExprZ e2)
+   | EPimpl e1 e2 => (interp_ExprP e1) -> (interp_ExprP e2)
+   | EPequiv e1 e2 => (interp_ExprP e1) <-> (interp_ExprP e2)
+   | EPand e1 e2 => (interp_ExprP e1) /\ (interp_ExprP e2)
+   | EPor e1 e2 => (interp_ExprP e1) \/ (interp_ExprP e2)
+   | EPneg e1 => ~ (interp_ExprP e1)
+   | EPraw p => p
+ end.
+
+Fixpoint norm_ExprZ (e:ExprZ) : ExprZ := 
+ match e with 
+  | EZraw z => EZraw z
+  | EZplus e1 e2 => EZplus (norm_ExprZ e1) (norm_ExprZ e2)
+  | EZminus e1 e2 => EZminus (norm_ExprZ e1) (norm_ExprZ e2)
+  | EZmult e1 e2 => EZmult (norm_ExprZ e1) (norm_ExprZ e2)
+  | EZmax e1 e2 => EZmax (norm_ExprZ e1) (norm_ExprZ e2)
+  | EZopp e1 => EZopp (norm_ExprZ e1)
+  | EZofI e1 =>  norm_ExprI_i2z e1
+ end
+with norm_ExprI_i2z (e:ExprI) : ExprZ := 
+ match e with 
+  | EI0 => EZraw (0%Z)
+  | EI1 => EZraw (1%Z)
+  | EI2 => EZraw (2%Z)
+  | EI3 => EZraw (3%Z) 
+  | EIplus e1 e2 => EZplus (norm_ExprI_i2z e1) (norm_ExprI_i2z e2)
+  | EIminus e1 e2 => EZminus (norm_ExprI_i2z e1) (norm_ExprI_i2z e2)
+  | EImult e1 e2 => EZmult (norm_ExprI_i2z e1) (norm_ExprI_i2z e2)
+  | EImax e1 e2 => EZmax (norm_ExprI_i2z e1) (norm_ExprI_i2z e2)
+  | EIopp e1 => EZopp (norm_ExprI_i2z e1)
+  | EIofZ e1 => norm_ExprZ e1
+  | EIraw i => EZofI (EIraw i) 
+ end.
+
+Fixpoint norm_ExprP (e:ExprP) : ExprP := 
+  match e with 
+   | EPeq e1 e2 => EPeq (norm_ExprZ e1) (norm_ExprZ e2)
+   | EPlt e1 e2 => EPlt (norm_ExprZ e1) (norm_ExprZ e2)
+   | EPle e1 e2 => EPle (norm_ExprZ e1) (norm_ExprZ e2)
+   | EPgt e1 e2 => EPgt (norm_ExprZ e1) (norm_ExprZ e2)
+   | EPge e1 e2 => EPge (norm_ExprZ e1) (norm_ExprZ e2)
+   | EPimpl e1 e2 => EPimpl (norm_ExprP e1) (norm_ExprP e2)
+   | EPequiv e1 e2 => EPequiv (norm_ExprP e1) (norm_ExprP e2)
+   | EPand e1 e2 => EPand (norm_ExprP e1) (norm_ExprP e2)
+   | EPor e1 e2 => EPor (norm_ExprP e1) (norm_ExprP e2)
+   | EPneg e1 => EPneg (norm_ExprP e1)
+   | EPraw p => EPraw p
+ end.
+
+Scheme ExprZ_mrec := Induction for ExprZ Sort Prop
+with ExprI_mrec := Induction for ExprI Sort Prop.
+
+Lemma norm_ExprIZ_correct : 
+  forall e:ExprZ, interp_ExprZ (norm_ExprZ e) = interp_ExprZ e.
+Proof.
+  set (P:= fun e => interp_ExprZ (norm_ExprZ e) = interp_ExprZ e).
+  set (Q:= fun e => interp_ExprZ (norm_ExprI_i2z e) = i2z (interp_ExprI e)).
+  apply (ExprZ_mrec P Q); unfold P, Q; simpl; intros; i2z; auto; try congruence.
+Qed. 
+
+Lemma norm_ExprP_correct : 
+  forall e:ExprP, interp_ExprP (norm_ExprP e) <-> interp_ExprP e.
+Proof.
+induction e; simpl; repeat (rewrite norm_ExprIZ_correct); intuition.
+Qed.
+
+Lemma norm_ExprP_correct2 : 
+  forall e:ExprP, interp_ExprP (norm_ExprP e) -> interp_ExprP e.
+Proof.
+intros; destruct (norm_ExprP_correct e); auto.
+Qed.
+
+Ltac i2z_refl := 
+  i2z_gen;
+  match goal with |- ?t => 
+     let e := interp_prop t 
+     in 
+     (change (interp_ExprP e); 
+      apply norm_ExprP_correct2; 
+      simpl)
+   end.
+
+Ltac iauto := i2z_refl; auto.
+Ltac iomega := i2z_refl; intros; romega.
+
+  Open Scope Z_scope.
 
   Lemma max_spec : forall (x y:Z), 
   x >= y /\ Zmax x y = x  \/
@@ -156,19 +410,23 @@ Module MoreInt (I:Int).
   destruct (Zcompare x y); [ left | right | left ]; split; auto; discriminate.
   Qed.
 
-  Ltac omega_max := i2z; 
-  let om x y := 
+  Ltac omega_max_genspec x y := 
     generalize (max_spec x y); 
     let z := fresh "z" in let Hz := fresh "Hz" in 
-    (set (z:=Zmax x y) in *; clearbody z; intro Hz)
-  in 
-  match goal with 
-    | |- context id [ Zmax ?x ?y ] => om x y; omega_max
-    | H:context id [ Zmax ?x ?y ] |- _ => om x y; omega_max
-    | _ => intros; try omega
-  end.
+    (set (z:=Zmax x y); clearbody z).
 
-  Ltac false_omega := elimtype False; iomega.
+  Ltac omega_max_loop := 
+    match goal with 
+      (* hack: we don't want [i2z (height ...)] to be reduced by romega later... *)
+      | |- context [ i2z (?f ?x) ] => 
+          let i := fresh "i2z" in (set (i:=i2z (f x)); clearbody i); omega_max_loop
+      | |- context [ Zmax ?x ?y ] => omega_max_genspec x y; omega_max_loop
+      | _ => intros
+    end.
+
+  Ltac omega_max := i2z_refl; omega_max_loop; try romega.
+
+  Ltac false_omega := elimtype False; i2z_refl; intros; romega.
   Ltac false_omega_max := elimtype False; omega_max.
 
  Open Scope Int_scope.
