FMapAVL.v
@@ -18,6 +18,8 @@ Require Import FSetInterface.
 Require Import FMapInterface.
 Require Import FMapList.
 
+Require Import ROmega.
+
 Require Import ZArith.
 Open Scope Z_scope.
 
@@ -36,22 +38,6 @@ Proof.
  intros; unfold max, Zle, Zge.
  destruct (Zcompare x y); [ left | right | left ]; split; auto; discriminate.
 Qed.
-
-Ltac omega_max := 
-  let om x y := 
-    generalize (max_spec x y); 
-    let z := fresh "z" in let Hz := fresh "Hz" in 
-    (set (z:=Zmax x y) in *; clearbody z; intro Hz)
-  in 
-  match goal with 
-    | |- context id [ max ?x ?y ] => om x y; omega_max
-    | H:context id [ max ?x ?y ] |- _ => om x y; omega_max
-    | _ => intros; try omega
-  end.
-
-Ltac false_omega := elimtype False; omega.
-Ltac false_omega_max := elimtype False; omega_max.
-
 
 
 Module Raw (X: OrderedType).
@@ -198,6 +184,29 @@ end.
 
 Ltac intuition_in := repeat progress (intuition; inv In; inv MapsTo).
 Ltac firstorder_in := repeat progress (firstorder; inv In; inv MapsTo).
+
+Ltac omega_max := 
+  let om x y := 
+    generalize (max_spec x y); 
+    let z := fresh "z" in let Hz := fresh "Hz" in 
+    (set (z:=Zmax x y) in *; clearbody z; intro Hz)
+  in 
+  let hei x := 
+     let h := fresh "h" in 
+     (set (h:=height x) in *; clearbody h)
+  in
+  (simpl in *; 
+  match goal with 
+    | |- context [ height ?x ] => hei x; omega_max
+    | H:context [ height ?x ] |- _ => hei x; omega_max
+    | |- context [ max ?x ?y ] => om x y; omega_max
+    | H:context [ max ?x ?y ] |- _ => om x y; omega_max
+    | _ => intros; try romega
+  end).
+
+Ltac false_omega := elimtype False; romega.
+Ltac false_omega_max := elimtype False; omega_max.
+
 
 Lemma height_non_negative : forall elt (s : t elt), avl s -> height s >= 0.
 Proof.
@@ -439,7 +448,7 @@ Ltac bal_tac :=
      | ]]; intros.
 
 Ltac bal_tac_imp := match goal with 
-  | |- context id [ assert_false ] => 
+  | |- context [ assert_false ] => 
       inv avl; avl_nns; simpl in *; false_omega
   | _ => idtac
 end.
@@ -486,7 +495,7 @@ Proof.
 Qed.
 
 Ltac omega_bal := match goal with 
-  | H:avl ?l, H':avl ?r |- context id [ bal ?l ?x ?e ?r ] => 
+  | H:avl ?l, H':avl ?r |- context [ bal ?l ?x ?e ?r ] => 
      generalize (bal_height_1 x e H H') (bal_height_2 x e H H'); 
      omega_max
   end. 
@@ -511,12 +520,12 @@ Proof.
  (* Lt *)
  destruct H; auto.
  split.
- apply bal_avl; auto; omega.
+ apply bal_avl; auto; omega_max.
  omega_bal.
  (* Gt *)
  destruct H; auto.
  split.
- apply bal_avl; auto; omega.
+ apply bal_avl; auto; omega_max.
  omega_bal.
 Qed.
 
@@ -723,7 +732,6 @@ Proof.
  apply bal_avl; auto.
  simpl; omega_max.
  omega_bal.
- simpl in *; omega_max.
 Qed.
 
 Lemma merge_avl : forall elt (s1 s2:t elt), avl s1 -> avl s2 -> 
@@ -1262,9 +1270,9 @@ Ltac Measure_e := unfold measure_e in |- *; fold measure_e in |- *.
 Lemma measure_e_t_0 : forall s : t elt, measure_e_t s >= 0.
 Proof.
  simple induction s.
- simpl in |- *; omega.
+ simpl in |- *; romega.
  intros.
- Measure_e_t; omega.
+ Measure_e_t; romega.
 Qed.
 
 Ltac Measure_e_t_0 s := generalize (@measure_e_t_0 s); intro.
@@ -1272,9 +1280,9 @@ Ltac Measure_e_t_0 s := generalize (@measure_e_t_0 s); intro.
 Lemma measure_e_0 : forall e : enumeration, measure_e e >= 0.
 Proof.
  simple induction e.
- simpl in |- *; omega.
+ simpl in |- *; romega.
  intros.
- Measure_e; Measure_e_t_0 t; omega.
+ Measure_e; Measure_e_t_0 t; romega.
 Qed.
 
 Ltac Measure_e_0 e := generalize (@measure_e_0 e); intro.
@@ -1299,7 +1307,7 @@ Proof.
             Zabs_nat (measure_e (fst xx') + measure_e (snd xx'))).
  intros; apply Zabs.Zabs_nat_lt.
  Measure_e_0 (fst x0); Measure_e_0 (snd x0); Measure_e_0 (fst y);
- Measure_e_0 (snd y); intros; omega.
+ Measure_e_0 (snd y); intros; romega.
 Qed.
 
 (** [cons t e] adds the elements of tree [t] on the head of 
@@ -1332,7 +1340,7 @@ Proof.
  destruct y; red; simpl in *; intuition.
  apply X.lt_trans with k; eauto.
  exists x; intuition.
- generalize H4; Measure_e; intros; Measure_e_t; omega.
+ generalize H4; Measure_e; intros; Measure_e_t; romega.
  rewrite H5.
  apply flatten_e_elements.
 Qed.
@@ -1381,7 +1389,7 @@ Proof.
  destruct (@cons t e0) as [c1 (H2,(H3,H4))]; try inversion_clear H0; auto.
  destruct (@cons t0 e4) as [c2 (H5,(H6,H7))]; try inversion_clear H1; auto.
  destruct (H c1 c2); clear H; intuition.
- Measure_e; omega.
+ Measure_e; romega.
  left.
  rewrite H4 in e6; rewrite H7 in e6.
  simpl; rewrite <- L.equal_cons; auto.
@@ -1985,7 +1993,7 @@ Module Make_ord (X: OrderedType)(D : OrderedType) <:
   assert (measure_e c1 + measure_e c2 <
               measure_e (More k t t0 e) + 
               measure_e (More k0 t1 t2 e0)).
-  unfold measure_e in *; fold measure_e in *; omega.           
+  unfold measure_e in *; fold measure_e in *; romega.           
   destruct (H c1 c2 H0 H2 H5); clear H.
   constructor 1.
   unfold flatten_slist, LO.lt in *; simpl; simpl in l.
